Work on polynomial interpretation

Code/Examples/Map.v
@@ -1,52 +1,186 @@
+Require Import Prelude.CompatibleRelation.
 Require Import Syntax.Signature.
+Require Import Syntax.StrongNormalization.SN.
+Require Import Interpretation.WeaklyMonotonicAlgebra.
+Require Import Interpretation.Polynomial.
+Require Import Interpretation.OrderInterpretation.
+
+Local Open Scope nat.
 
 Inductive base_types : Type :=
-| Nat   : base_types
-| List  : base_types.
+| TNat   : base_types
+| TList  : base_types.
+
+Definition Nat : ty base_types := Base TNat.
+Definition List : ty base_types := Base TList.
 
 Inductive fun_symbols : Type :=
-| Zero  : fun_symbols
-| Succ  : fun_symbols
-| Nil   : fun_symbols
-| Cons  : fun_symbols
-| Map   : fun_symbols.
+| TZero  : fun_symbols
+| TSucc  : fun_symbols
+| TNil   : fun_symbols
+| TCons  : fun_symbols
+| TMap   : fun_symbols.
 
 Definition map_ar
            (f : fun_symbols)
   : ty base_types
   := match f with
-     | Zero  => Base Nat
-     | Succ  => Base Nat ⟶ Base Nat
-     | Nil   => Base List
-     | Cons  => Base Nat ⟶ Base List ⟶ Base List
-     | Map   => (Base Nat ⟶ Base Nat) ⟶ Base List ⟶ Base List
+     | TZero  => Nat
+     | TSucc  => Nat ⟶ Nat
+     | TNil   => List
+     | TCons  => Nat ⟶ List ⟶ List
+     | TMap   => (Nat ⟶ Nat) ⟶ List ⟶ List
      end.
+
+Definition Zero
+           {C : con base_types}
+  : tm map_ar C Nat
+  := BaseTm TZero.
+
+Definition Suc
+           {C : con base_types}
+  : tm map_ar C (Nat ⟶ Nat)
+  := BaseTm TSucc.
+
+Definition Nil
+           {C : con base_types}
+  : tm map_ar C List
+  := BaseTm TNil.
+
+Definition Cons
+           {C : con base_types}
+  : tm map_ar C (Nat ⟶ List ⟶ List)
+  := BaseTm TCons.
+
+Definition Map
+           {C : con base_types}
+  : tm map_ar C ((Nat ⟶ Nat) ⟶ List ⟶ List)
+  := BaseTm TMap.
 
 Definition map_nil
   : rewriteRule map_ar
   := make_rewrite
-       ((Base Nat ⟶ Base Nat) ,, ∙)
-       (Base List)
+       ((Nat ⟶ Nat) ,, ∙)
+       List
        (let f := TmVar Vz in
-        BaseTm Map · f · BaseTm Nil : tm map_ar _ _)
-       (BaseTm Nil).
+        Map · f · Nil)
+       Nil.
 
 Definition map_cons
   : rewriteRule map_ar
   := make_rewrite
-       ((Base Nat ⟶ Base Nat) ,, Base Nat ,, Base List ,, ∙)
-       (Base List)
+       ((Nat ⟶ Nat) ,, Nat ,, List ,, ∙)
+       List
        (let f := TmVar Vz in
         let x := TmVar (Vs Vz) in
         let xs := TmVar (Vs (Vs Vz)) in
-        BaseTm Map · f · (BaseTm Cons · x · xs))
+        Map · f · (Cons · x · xs))
        (let f := TmVar Vz in
         let x := TmVar (Vs Vz) in
         let xs := TmVar (Vs (Vs Vz)) in
-        BaseTm Cons · (f · x) · (BaseTm Map · f · xs)).
+        Cons · (f · x) · (Map · f · xs)).
 
 Definition map_afs
   : afs base_types fun_symbols
   := make_afs
        map_ar
        (map_nil :: map_cons :: nil).
+
+Open Scope poly_scope.
+
+Definition map_fun_poly
+           (f : fun_symbols)
+  : poly ∙ (arity map_afs f)
+  := match f with
+     | TZero =>
+       P_base (P_const 1)
+     | TSucc =>
+       λP
+       let x := P_var Vz in
+       P_base (from_poly x +P P_const 1)
+     | TNil =>
+       P_base (P_const 1)
+     | TCons =>
+       λP
+       let x := P_var Vz in
+       λP
+       let xs := P_var (Vs Vz) in
+       P_base (P_const 1 +P (from_poly x +P from_poly xs))
+     | TMap =>
+       λP
+       let xs := P_var Vz in
+       λP
+       let f := P_var (Vs Vz) in
+       P_base (P_const 1 +P ((P_const 1 +P from_poly xs) *P from_poly (f ·P P_base (from_poly xs))))
+     end.
+
+Close Scope poly_scope.
+
+(*
+Notation "0" := (P_const 0).
+Notation "1" := (P_const 1).
+Notation "2" := (P_const 2).
+Notation "3" := (P_const 3).
+
+Definition map_fun_poly
+  : forall f : fun_symbols, poly ∙ (arity map_afs f)
+  := fun f =>
+     match f with
+     | TZero =>
+       P_base 1
+     | TSucc =>
+       λP
+       let x := P_var Vz in
+       P_base (from_poly x +P 1)
+     | TNil =>
+       P_base 1
+     | TCons =>
+       λP
+       let x := P_var Vz in
+       λP
+       let xs := P_var (Vs Vz) in
+       P_base (1 +P (from_poly x +P from_poly xs))
+     | TMap =>
+       λP
+       let xs := P_var Vz in
+       λP
+       let f := P_var (Vs Vz) in
+       P_base (1 +P ((1 +P from_poly xs) *P from_poly (f ·P P_base (from_poly xs))))
+     end.
+ *)
+
+(*
+Definition map_isSN
+  : isSN map_afs.
+Proof.
+  apply afs_is_SN_from_Alg.
+  simple refine (poly_WMalgebra _ _ _ _ _ _ _).
+  - exact map_fun_poly.
+  - intros A1 A2.
+    refine (P_app _ _).
+    + apply P_var.
+      apply Vz.
+    + apply P_var.
+      apply Vs.
+      apply Vz.
+  - intros A1 A2 f x.
+    cbn.
+    apply ge_refl.
+  - intros A1 A2 f1 f2 x Hf.
+    cbn.
+    apply Hf.
+  - intros A1 A2 f x1 x2 Hx.
+    cbn.
+    admit.
+  - intros r x.
+    cbn in *.
+    destruct r as [ r Hr ].
+    repeat (destruct Hr as [ | Hr ]) ; try subst ; cbn in *.
+    + destruct x ; cbn in *.
+      admit.
+    + destruct x as [ f [ x1 [ x2 [ ] ] ] ].
+      nia.
+      admit.
+    + contradiction.
+Admitted.
+ *)
