Code/Interpretation/Polynomial.v
@@ -1,0 +1,348 @@
+Require Import Prelude.Funext.
+Require Import Prelude.WellfoundedRelation.
+Require Import Prelude.CompatibleRelation.
+Require Import Prelude.Lexico.
+Require Import Syntax.Signature.
+Require Import Syntax.StrongNormalization.SN.
+Require Import Syntax.StrongNormalization.BetaReductionSN.
+Require Import Interpretation.OrderInterpretation.
+Require Import Interpretation.WeaklyMonotonicAlgebra.
+
+Declare Scope poly_scope.
+
+Inductive base_poly {B : Type} : con B -> Type :=
+| P_const : forall {C : con B}, nat -> base_poly C
+| P_plus : forall {C : con B}, base_poly C -> base_poly C -> base_poly C
+| P_mult : forall {C : con B}, base_poly C -> base_poly C -> base_poly C
+| from_poly : forall {C : con B} {b : B},
+                poly C (Base b)
+                -> base_poly C
+with poly {B : Type} : con B -> ty B -> Type :=
+| P_base : forall {C : con B} {b : B}, base_poly C -> poly C (Base b)
+| P_var : forall {C : con B} {A : ty B},
+            var C A
+            -> poly C A
+| P_app : forall {C : con B} {A₁ A₂ : ty B},
+            poly C (A₁ ⟶ A₂)
+            -> poly C A₁
+            -> poly C A₂
+| P_lam : forall {C : con B} {A₁ A₂ : ty B},
+            poly (A₁ ,, C) A₂
+            -> poly C (A₁ ⟶ A₂).
+
+Notation "P1 +P P2" := (P_plus P1 P2) (at level 50) : poly_scope.
+Notation "P1 *P P2" := (P_mult P1 P2) (at level 40) : poly_scope.
+Notation "'λP' P" := (P_lam P) (at level 10) : poly_scope.
+Notation "P1 ·P P2" := (P_app P1 P2) (at level 20) : poly_scope.
+
+Fixpoint sem_base_poly
+         {B : Type}
+         {C : con B}
+         (P : base_poly C)
+  : weakMonotoneMap
+      (sem_Con (fun _ => nat_CompatRel) C)
+      nat_CompatRel
+  := match P with
+     | P_const n   => const_WM _ nat_CompatRel n
+     | P_plus P1 P2  => plus_WM (sem_base_poly P1) (sem_base_poly P2)
+     | P_mult P1 P2  => mult_WM (sem_base_poly P1) (sem_base_poly P2)
+     | from_poly P   => sem_poly P
+     end
+with sem_poly
+      {B : Type}
+      {C : con B}
+      {A : ty B}
+      (P : poly C A)
+  : weakMonotoneMap
+      (sem_Con (fun _ => nat_CompatRel) C)
+      (sem_Ty (fun _ => nat_CompatRel) A)
+  := match P with 
+     | P_base P   => sem_base_poly P
+     | P_var v      => sem_Var (fun _ => nat_CompatRel) v
+     | P_app P1 P2  => app_WM (sem_poly P1) (sem_poly P2)
+     | P_lam P      => lambda_abs (sem_poly P)
+     end.
+
+Notation "⟦ P ⟧" := (sem_poly P).
+Notation "⟦ P ⟧B" := (sem_base_poly P).
+
+Definition prod_unit_map
+           (A B : CompatRel)
+  : weakMonotoneMap (A * B) (A * (B * unit_CompatRel)).
+Proof.
+  unshelve esplit.
+  - exact (fun z => (fst z , (snd z , tt))).
+  - intros z1 z2 p ; cbn.
+    repeat split ; auto.
+    + apply p.
+    + apply p.
+Defined.
+
+Section PolyAlgebra.
+  Context {B : Type} {F : Type}
+          (X : afs B F)
+          (P : forall (f : F), poly ∙ (arity X f))
+          (app : forall (A1 A2 : ty B), poly ((A1 ⟶ A2) ,, A1 ,, ∙) A2).
+
+  Definition p_base : B -> CompatRel
+    := fun _ : B => nat_CompatRel.
+
+  Definition p_tm (f : F) : sem_Ty p_base (arity X f)
+    := sem_poly (P f) tt.
+
+  Definition p_app (A1 A2 : ty B)
+    := comp_WM
+         (prod_unit_map
+            (sem_Ty p_base (A1 ⟶ A2))
+            (sem_Ty p_base A1))
+         (sem_poly (app A1 A2)).
+  
+  Definition poly_WMalgebra
+             (H1 : forall (A1 A2 : ty B)
+                          (f : weakMonotoneMap (sem_Ty p_base A1) (sem_Ty p_base A2))
+                          (x : sem_Ty p_base A1),
+                 ⟦ app A1 A2 ⟧ (f , (x , tt)) >= f x)
+             (H2 : forall (A1 A2 : ty B)
+                          (f1 f2 : weakMonotoneMap (sem_Ty p_base A1) (sem_Ty p_base A2))
+                          (x : sem_Ty p_base A1),
+                 (forall z, f1 z > f2 z)
+                 ->
+                 ⟦ app A1 A2 ⟧ (f1, (x, tt))
+                 >
+                 ⟦ app A1 A2 ⟧ (f2 , (x , tt)))
+             (H3 : forall (A1 A2 : ty B)
+                          (f : weakMonotoneMap (sem_Ty p_base A1) (sem_Ty p_base A2))
+                          (x1 x2 : sem_Ty p_base A1),
+                 x1 > x2
+                 ->
+                 ⟦ app A1 A2 ⟧ (f , (x1 , tt))
+                 >
+                 ⟦ app A1 A2 ⟧ (f , (x2 , tt)))
+             (H4 : forall (r : rewriteRules X)
+                          (x : sem_Con p_base (vars r)),
+                 sem_Tm p_base p_tm p_app (lhs r) x
+                 >
+                 sem_Tm p_base p_tm p_app (rhs r) x)
+    : WMalgebra X.
+  Proof.
+    simple refine (make_WMalgebra
+                     X
+                     p_base
+                     (fun _ => 0)
+                     (fun _ => nat_Wf)
+                     _
+                     p_tm
+                     p_app
+                     H1 H2 H3 _).
+    - intros r C s x.
+      rewrite !sub_Lemma.
+      apply H4.
+  Defined.
+End PolyAlgebra.
+
+
+(*
+Inductive base_poly {B : Type} : con B -> Type :=
+| P_const : forall (C : con B), nat -> base_poly C
+| P_plus : forall (C : con B), base_poly C -> base_poly C -> base_poly C
+| P_mult : forall (C : con B), base_poly C -> base_poly C -> base_poly C
+| P_b_app : forall (C : con B) (A : ty B) (b : B),
+              poly C (A ⟶ Base b)
+              -> poly C A
+              -> base_poly C
+| P_b_var : forall (C : con B) (b : B), var C (Base b) -> base_poly C
+with poly {B : Type} : con B -> ty B -> Type :=
+| P_base : forall (C : con B) (b : B), base_poly C -> poly C (Base b)
+| P_var : forall (C : con B) (A : ty B),
+            var C A
+            -> poly C A
+| P_app : forall (C : con B) (A₁ A₂ : ty B),
+            poly C (A₁ ⟶ A₂)
+            -> poly C A₁
+            -> poly C A₂
+| P_lam : forall (C : con B) (A₁ A₂ : ty B),
+            poly (A₁ ,, C) A₂
+            -> poly C (A₁ ⟶ A₂).
+*)
+(*
+Inductive poly {B : Type} : con B -> ty B -> Type :=
+| P_const : forall (C : con B) (b : B),
+              nat -> poly C (Base b)
+| P_plus : forall (C : con B) (b₁ b₂ b₃ : B),
+              poly C (Base b₁)
+              -> poly C (Base b₂)
+              -> poly C (Base b₃)
+| P_mult : forall (C : con B) (b₁ b₂ b₃ : B),
+              poly C (Base b₁)
+              -> poly C (Base b₂)
+              -> poly C (Base b₃)
+| P_var : forall (C : con B) (A : ty B),
+            var C A
+            -> poly C A
+| P_app : forall (C : con B) (A₁ A₂ : ty B),
+            poly C (A₁ ⟶ A₂)
+            -> poly C A₁
+            -> poly C A₂
+| P_lam : forall (C : con B) (A₁ A₂ : ty B),
+            poly (A₁ ,, C) A₂
+            -> poly C (A₁ ⟶ A₂).
+
+
+Definition sem_poly
+         {B : Type}
+         {C : con B}
+         {A : ty B}
+         (P : poly C A)
+  : weakMonotoneMap
+      (sem_Con (fun _ => nat_CompatRel) C)
+      (sem_Ty (fun _ => nat_CompatRel) A).
+Proof.
+  induction P.
+  - apply (const_WM _ nat_CompatRel n).
+  - apply (plus_WM IHP1 IHP2).
+  - apply (mult_WM IHP1 IHP2).
+  - apply (sem_Var (fun _ => nat_CompatRel) v).
+  - apply (app_WM IHP1 IHP2).
+  - apply (lambda_abs IHP).
+Defined.
+
+(*
+Inductive poly {B : Type} : con B -> ty B -> Type :=
+| P_const   : forall (C : con B) (b : B),
+                nat -> poly C (Base b)
+| P_plus    : forall {C : con B} {b : B},
+                poly C (Base b)
+                -> poly C (Base b)
+                -> poly C (Base b)
+| P_mult    : forall {C : con B} {b : B},
+                poly C (Base b)
+                -> poly C (Base b)
+                -> poly C (Base b)
+| P_base    : forall {C : con B} {b : B},
+                base_poly C (Base b)
+                -> poly C (Base b)
+| P_lam     : forall {C : con B} {A1 A2 : ty B},
+                poly (A1 ,, C) A2
+                -> poly C (A1 ⟶ A2)
+with base_poly {B : Type} : con B -> ty B -> Type :=
+| PVar      : forall {C : con B} {A : ty B},
+                var C A
+                -> base_poly C A
+| Papp      : forall {C : con B} {A B : ty B},
+                base_poly C (A ⟶ B)
+                -> poly C A
+                -> base_poly C B.
+
+Fixpoint sem_poly
+         {B : Type}
+         {C : con B}
+         {A : ty B}
+         (P : poly C A)
+  : weakMonotoneMap
+      (sem_Con (fun _ => nat_CompatRel) C)
+      (sem_Ty (fun _ => nat_CompatRel) A)
+  := match P with
+     | P_const _ _ n  => const_WM _ nat_CompatRel n
+     | P_plus P1 P2   => plus_WM (sem_poly P1) (sem_poly P2)
+     | P_mult P1 P2   => mult_WM (sem_poly P1) (sem_poly P2)
+     | P_base P       => sem_base_poly P
+     | P_lam P        => lambda_abs (sem_poly P)
+     end
+with sem_base_poly
+     {B : Type}
+     {C : con B}
+     {A : ty B}
+     (P : base_poly C A)
+  : weakMonotoneMap
+      (sem_Con (fun _ => nat_CompatRel) C)
+      (sem_Ty (fun _ => nat_CompatRel) A)
+  := match P with
+     | PVar v         => sem_Var (fun _ => nat_CompatRel) v
+     | Papp P1 P2     => app_WM (sem_base_poly P1) (sem_poly P2)
+     end.
+
+Definition prod_unit_map
+           (A B : CompatRel)
+  : weakMonotoneMap (A * B) (A * (B * unit_CompatRel)).
+Proof.
+  unshelve esplit.
+  - exact (fun z => (fst z , (snd z , tt))).
+  - intros z1 z2 p ; cbn.
+    repeat split ; auto.
+    + apply p.
+    + apply p.
+Defined.
+  
+Definition poly_WMalgebra
+           {B : Type} {F : Type}
+           (X : afs B F)
+           (P : forall (f : F), poly ∙ (arity X f))
+           (app : forall (A1 A2 : ty B), poly ((A1 ⟶ A2) ,, A1 ,, ∙) A2)
+           (H1 : forall (A1 A2 : ty B)
+                        (f : weakMonotoneMap
+                               (sem_Ty (fun _ : B => nat_CompatRel) A1)
+                               (sem_Ty (fun _ : B => nat_CompatRel) A2))
+                        (x : sem_Ty (fun _ : B => nat_CompatRel) A1),
+               sem_poly (app A1 A2) (f, (x, tt)) >= f x)
+           (H2 : forall (A1 A2 : ty B)
+                        (f1 f2 : weakMonotoneMap
+                                   (sem_Ty (fun _ : B => nat_CompatRel) A1)
+                                   (sem_Ty (fun _ : B => nat_CompatRel) A2))
+                        (x : sem_Ty (fun _ : B => nat_CompatRel) A1),
+               (forall z, f1 z > f2 z)
+               ->
+               sem_poly (app A1 A2) (f1, (x, tt))
+               >
+               sem_poly (app A1 A2) (f2 , (x , tt)))
+           (H3 : forall (A1 A2 : ty B)
+                        (f : weakMonotoneMap
+                               (sem_Ty (fun _ : B => nat_CompatRel) A1)
+                               (sem_Ty (fun _ : B => nat_CompatRel) A2))
+                        (x1 x2 : sem_Ty (fun _ : B => nat_CompatRel) A1),
+               x1 > x2
+               ->
+               sem_poly (app A1 A2) (f, (x1, tt))
+               >
+               sem_poly (app A1 A2) (f, (x2, tt)))
+           (H4 : forall (r : rewriteRules X)
+                        (x : sem_Con (fun _ : B => nat_CompatRel) (vars r)),
+               sem_Tm
+                 (fun _ : B => nat_CompatRel)
+                 (fun f : F => sem_poly (P f) tt)
+                 (fun A1 A2 : ty B =>
+                    comp_WM
+                      (prod_unit_map
+                         (sem_Ty (fun _ : B => nat_CompatRel) (A1 ⟶ A2))
+                         (sem_Ty (fun _ : B => nat_CompatRel) A1))
+                      (sem_poly (app A1 A2)))
+                 (lhs r)
+                 x
+               >
+               sem_Tm
+                 (fun _ : B => nat_CompatRel)
+                 (fun f : F => sem_poly (P f) tt)
+                 (fun A1 A2 : ty B =>
+                    comp_WM
+                      (prod_unit_map
+                         (sem_Ty (fun _ : B => nat_CompatRel) (A1 ⟶ A2))
+                         (sem_Ty (fun _ : B => nat_CompatRel) A1))
+                      (sem_poly (app A1 A2)))
+                 (rhs r)
+                 x)
+  : WMalgebra X.
+Proof.
+  simple refine (make_WMalgebra
+                   X
+                   (fun _ => nat_CompatRel)
+                   (fun _ => 0)
+                   (fun _ => nat_Wf)
+                   _
+                   (fun f => sem_poly (P f) tt)
+                   (fun A1 A2 => comp_WM (prod_unit_map _ _) (sem_poly (app A1 A2)))
+                   H1 H2 H3 _).
+  - intros r C s x.
+    rewrite !sub_Lemma.
+    apply H4.
+Defined.
+ *)
+ *)
